stlc_cont_ty transform qed

stlc_cont_ty.v
@@ -45,9 +45,9 @@ Inductive ty: Type :=
 
 Definition tenv := list ty.
 
-(* \gamma, current continuation capability |- tm : ty *)
+(* \gamma, most recently introduced continuation capability |- tm : ty *)
 Inductive has_type : tenv -> (option ty) -> tm -> ty -> Type := 
-  (* values *)
+  (* Values *)
   | t_true : forall env K, 
       has_type env K ttrue TBool
   
@@ -66,7 +66,7 @@ Inductive has_type : tenv -> (option ty) -> tm -> ty -> Type :=
       has_type (T1 :: env) (Some R) t T2 -> 
       has_type env K (tcontabs t) (TKFun T1 R T2)
 
-  (* redexes *)
+  (* Redexes *)
   | t_if : forall env K cond tbranch ebranch T,
       has_type env K cond TBool -> 
       has_type env K tbranch T -> 
@@ -115,22 +115,283 @@ Fixpoint trans_env(env: tenv): B.tenv :=
 #[export] Hint Constructors tm: core.
 #[local] Hint Constructors B.has_type : core.
 
-(* Fixpoint transform { env K t T } (H : has_type env K t T) : B.tm := 
-match H in (has_type _ _ _ _) return B.tm with 
-  | t_true _ _ => B.ttrue
-  | t_false _ _ => B.tfalse
-  | t_var env R x T H => B.tvar x
-  | t_abs env R t T1 T2 HT =>
-    B.tabs (transform3 HT)
+Fixpoint transform { env K t T } (H : has_type env K t T) : B.tm * bool := 
+match H in (has_type _ _ _ _) return (B.tm * bool) with 
+  (* Values *)
+  | t_true _ _ => (B.ttrue, false)
+  | t_false _ _ => (B.tfalse, false)
+  | t_var env K x T H => (B.tvar x, false)
+  
+  | t_abs env K t T1 T2 HT => 
+    (B.tabs (fst (transform HT)), false)
 
-  | t_if env R cond tbranch ebranch T HTC HTT HTE =>
-    B.tif (transform3 HTC) (transform3 HTT) (transform3 HTE)
+  | t_contabs env K t T1 R T2 HT => 
+    let (rt, bt) := transform HT in 
+    if bt then 
+      (B.tabs (B.tabsk (B.tapp rt (B.tvark 0))), false)
+    else 
+      (B.tabs (B.tabsk (B.tapp (B.tvark 0) rt)), false)
 
-  | t_app env R f t T1 T2 HF HT =>  
-    B.tapp (transform3 HF) (transform3 HT)
+  (* Redexes *)
+  | t_if env K cond tbranch ebranch T HTC HTT HTE =>
+    let (rc, bc) := (transform HTC) in 
+    let (rt, bt) := (transform HTT) in 
+    let (re, be) := (transform HTE) in 
+    match (bc, bt, be) with 
+    | (false, false, false) => (B.tif rc rt re, false)
+    | (true, false, false) => (B.tabsk
+        (B.tapp rc (B.tabsk (B.tif (B.tvark 0) 
+          (B.tapp (B.tvark 1) rt)
+          (B.tapp (B.tvark 1) re)
+        ))), true)
+    | (false, true, false) => (B.tabsk (
+        B.tif rc 
+        (B.tapp rt (B.tvark 0))
+        (B.tapp (B.tvark 0) re)
+      ), true)
+    | (true, true, false) => (B.tabsk (
+        B.tapp rc (B.tabsk (B.tif (B.tvark 0) 
+          (B.tapp rt (B.tvark 1))
+          (B.tapp (B.tvark 1) re)
+        ))
+      ), true)
+    | (false, false, true) => (B.tabsk (
+        B.tif rc 
+        (B.tapp (B.tvark 0) rt)
+        (B.tapp re (B.tvark 0))
+    ), true)
+    | (true, false, true) => (B.tabsk (
+        B.tapp rc (B.tabsk (B.tif (B.tvark 0)
+          (B.tapp (B.tvark 1) rt)
+          (B.tapp re (B.tvark 1))
+        ))
+    ), true) 
+    | (false, true, true) => (B.tabsk (
+        B.tif rc 
+        (B.tapp rt (B.tvark 0))
+        (B.tapp re (B.tvark 0))
+    ), true)
+    | (true, true, true) => (B.tabsk (
+        B.tapp rc (B.tabsk (B.tif (B.tvark 0)
+          (B.tapp rt (B.tvark 1))
+          (B.tapp re (B.tvark 1))
+        ))
+    ), true)
+    end
 
-  | _ => id_abs
-end. *)
+  | t_app env K f t T1 T2 HF HT =>  
+    let (rf, bf) := (transform HF) in 
+    let (rt, bt) := (transform HT) in 
+    match (bf, bt) with 
+    | (false, false) => (B.tapp rf rt, false)
+
+    | (true, false) => ( B.tabsk (
+      B.tapp rf (B.tabsk (
+        B.tapp (B.tvark 1) (
+          B.tapp (B.tvark 0) rt
+        )
+      ))
+    ), true)
+    | (false, true) => (B.tabsk (
+        B.tapp rt (B.tabsk (
+          B.tapp (B.tvark 1) (
+            B.tapp rf (B.tvark 0)
+          )
+        ))
+    ), true)
+    | (true, true) => (B.tabsk (
+        B.tapp rf ( B.tabsk (
+          B.tapp rt ( B.tabsk (
+            B.tapp (B.tvark 2)
+            (B.tapp (B.tvark 1) (B.tvark 0))
+          )) 
+        ))
+    ), true)
+    end 
+
+  | t_reset env K t R HT => 
+    let (rt, bt) := transform HT in 
+    if bt then 
+      (B.tapp rt (B.tabs (B.tvar 0)), false)
+    else 
+      (rt, false)
+
+  | t_shift env t A R HT => 
+    (B.tabs (fst (transform HT)),true) 
+
+  | t_contapp env f t T1 R T2 HF HT => 
+    let (rf, bf) := (transform HF) in 
+    let (rt, bt) := (transform HT) in 
+    match (bf, bt) with 
+    | (false, false) => (B.tabsk (
+        B.tapp (B.tapp rf rt) 
+        (B.tvark 0)
+      ), true)
+    | (true, false) => (B.tabsk (
+        B.tapp rf ( B.tabsk (
+          B.tapp (B.tapp (B.tvark 0) rt)
+          (B.tvark 1)
+        ))
+    ), true)
+    | (false, true) => (B.tabsk (
+        B.tapp rt (B.tabsk (
+          B.tapp (B.tapp (rf) (B.tvark 0)) 
+          (B.tvark 1)
+        ))
+    ), true) 
+    | (true, true) => (B.tabsk (
+        B.tapp rf (B.tabsk (
+          B.tapp rt (B.tabsk (
+            B.tapp (B.tapp (B.tvark 1) (B.tvark 0))
+            (B.tvark 2)
+          ))
+        )) 
+    ), true)
+    end
+end.
+
+Theorem fundamental : forall env K t T (H: has_type env K t T) t' b kenv,
+  (t', b) = transform H -> 
+  match K with 
+  | None => 
+    b = false /\
+    B.has_type (trans_env env) kenv t' (trans_ty T)
+  | Some R => 
+    if b then 
+      forall k,
+      B.has_type (trans_env env) kenv k (B.TFun (trans_ty T) (trans_ty R)) -> 
+      B.has_type (trans_env env) kenv (B.tapp t' k) (trans_ty R)
+    else 
+      B.has_type (trans_env env) kenv t' (trans_ty T)
+  end.
+Proof. 
+  intros env K t T H. induction H; 
+  intros t' b kenv HB; try (destruct K as [ Ans |]). 
+  (* t_true *)
+  - inversion HB. constructor.
+  - inversion HB. split; auto.
+  (* t_false *) 
+  - inversion HB. constructor.
+  - inversion HB. split; auto.
+  (* t_var *)
+  - inversion HB. constructor. apply indexl_map. apply e.
+  - inversion HB. split. reflexivity. constructor. apply indexl_map. apply e.
+  (* t_abs *)    
+  - simpl in *. inversion HB. destruct (transform H).    
+    destruct (IHhas_type t0 b0 kenv eq_refl). subst. auto.
+  - simpl in *. inversion HB. destruct (transform H). 
+    destruct (IHhas_type t0 b0 kenv eq_refl). subst. split; auto.
+  (* t_contabs *)
+  - simpl in *. destruct (transform H) as (r & br).
+    specialize (IHhas_type r br (B.TFun (trans_ty T2) (trans_ty R) :: kenv) eq_refl). 
+    destruct br; inversion HB; eauto.
+    + econstructor. econstructor. econstructor; eauto. repeat econstructor.
+  - simpl in *. destruct (transform H) as (r & br). 
+    specialize (IHhas_type r br (B.TFun (trans_ty T2) (trans_ty R) :: kenv) eq_refl).
+    destruct br; inversion HB; split; eauto.
+    + constructor. constructor. econstructor; eauto. repeat econstructor.
+  (* t_if *)
+  - simpl in *. 
+    destruct (transform H) as (rc & bc).
+    destruct (transform H0) as (rt & bt). 
+    destruct (transform H1) as (re & be).
+    specialize (IHhas_type1 rc bc). 
+    specialize (IHhas_type2 rt bt).
+    specialize (IHhas_type3 re be).
+    destruct bc; destruct bt; destruct be; inversion HB; try (intros k HK).
+    (* (true, true, true) *)
+    + econstructor; eauto. constructor. apply IHhas_type1; eauto.
+      do 2 constructor; eauto. 
+    (* (true, true, false) *)
+    + econstructor; eauto. constructor. apply IHhas_type1; auto.
+      do 2 constructor; eauto. repeat econstructor. eauto.
+    (* (true, false, true) *)
+    + econstructor; eauto. constructor. apply IHhas_type1; auto.
+      do 2 constructor; auto. repeat econstructor. eauto.
+    (* (true, false, false) *)
+    + econstructor; eauto. constructor. apply IHhas_type1; auto.
+      repeat econstructor; eauto.
+    (* (false, true, true) *)
+    + econstructor; eauto. do 2 constructor; eauto.
+    (* (false, true, false) *)
+    + econstructor; eauto. do 2 constructor; eauto. repeat econstructor. eauto.
+    (* (false, false, true )*)
+    + econstructor; eauto. do 2 constructor; eauto. repeat econstructor. eauto.
+    + eauto.
+  - simpl in *.     
+    destruct (transform H) as (rc & bc). 
+    destruct (transform H0) as (rt & bt). 
+    destruct (transform H1) as (re & be). 
+    destruct (IHhas_type1 rc bc kenv eq_refl). subst. 
+    destruct (IHhas_type2 rt bt kenv eq_refl). subst. 
+    destruct (IHhas_type3 re be kenv eq_refl). subst. 
+    inversion HB. split; simpl; auto. 
+  (* t_app *)
+  - simpl in *.
+    destruct (transform H) as (rf & bf).
+    destruct (transform H0) as (rt & bt).
+    specialize (IHhas_type1 rf bf).
+    specialize (IHhas_type2 rt bt). 
+    destruct bf; destruct bt; inversion HB; try (intros k HK).  
+    (* (true, true) *)
+    + econstructor; eauto. constructor. apply IHhas_type1; eauto.
+      constructor. apply IHhas_type2; eauto. repeat econstructor.
+    (* (true, false) *)
+    + econstructor; eauto. constructor. apply IHhas_type1; eauto.
+      repeat econstructor. auto.
+    + econstructor; eauto. constructor. apply IHhas_type2; eauto.
+      repeat econstructor. auto.
+    + eauto.
+  - simpl in *. 
+    destruct (transform H) as (rf & bf).
+    destruct (transform H0) as (rt & bt).
+    destruct (IHhas_type1 rf bf kenv eq_refl). 
+    destruct (IHhas_type2 rt bt kenv eq_refl). subst.
+    inversion HB. split; econstructor; eauto.
+  (* t_reset *)
+  - simpl in *. destruct (transform H) as (r & br).
+    specialize (IHhas_type r br kenv eq_refl). destruct br; inversion HB;
+    apply IHhas_type. repeat econstructor.
+  - simpl in *. destruct (transform H) as (r & br).
+    specialize (IHhas_type r br kenv eq_refl). destruct br; inversion HB; auto.
+  (* t_shift *)
+  - simpl in *. inversion HB. intros k HK. econstructor; eauto. econstructor.
+    destruct (transform H). specialize (IHhas_type t0 b0 kenv eq_refl).
+    apply IHhas_type. 
+  (* t_contapp *)
+  - simpl in *.    
+    destruct (transform H) as (rf & bf).
+    destruct (transform H0) as (rt & bt).
+    specialize (IHhas_type1 rf bf). 
+    specialize (IHhas_type2 rt bt).
+    destruct bf; destruct bt; inversion HB; try (intros K HK).
+    (* (true, true) *)
+    + econstructor; eauto. constructor. apply IHhas_type1; eauto.
+      constructor. apply IHhas_type2. auto. repeat econstructor.
+    (* (true, false) *)
+    + econstructor; eauto. constructor. apply IHhas_type1; eauto.
+      repeat econstructor. eauto.
+    (* (false, true) *)
+    + econstructor; eauto. constructor. apply IHhas_type2; eauto.
+      repeat econstructor. eauto.
+    + repeat econstructor; eauto.
+Qed.
+
+Theorem transl_pre_types: forall t T (H: has_type [] None t T),
+  B.has_type [] [] (fst (transform H)) (trans_ty T).
+Proof.
+  intros t T H. remember (transform H) as res. 
+  destruct (res) as (t' & b). 
+  pose proof (fundamental _ _ _ _ H t' b []) as HQ.
+  simpl in *. rewrite <- Heqres in HQ. apply HQ.
+  reflexivity.
+Qed.   
+
+Corollary safety : forall t T (H: has_type [] None t T), 
+  B.exp_type [] [] (fst (transform H)) (trans_ty T).
+Proof.
+  intros. apply B.safety. apply transl_pre_types.
+Qed.
 
 End STLC_CONT_TY.
 
